instr.v
@@ -1,0 +1,35 @@
+Require Import Resources.utility.
+Require Import Resources.name.
+Require Import Resources.type.
+Require Import Resources.value.
+
+(** Move Instructions *)
+Inductive OpCode : Set.
+
+Parameter op_arity : OpCode → nat → Prop.
+
+Parameter legal : OpCode → list UnrestrictedValue → Prop.
+
+Parameter opcode_to_op: OpCode → list UnrestrictedValue → UnrestrictedValue.
+
+Inductive Instr : Set :=
+  | MvLoc : LocalVariable → Instr
+  | CpLoc : LocalVariable → Instr
+  | StLoc : LocalVariable → Instr
+  | BorrowLoc : LocalVariable → Instr
+  | BorrowField : FieldName → Instr
+  | FreezeRef : Instr
+  | ReadRef : Instr
+  | WriteRef : Instr
+  | Pop : Instr
+  | Pack : StructType → Instr
+  | Unpack : Instr
+  | LoadTrue : Instr
+  | LoadFalse : Instr
+  | LoadU64 : UnsignedInt64 → Instr
+  | LoadAddress : AccountAddress → Instr
+  | LoadBytes : Bytes → Instr
+  | Op : OpCode → Instr
+.
+
+Coercion Op : OpCode >-> Instr.
