memory.v
@@ -1,0 +1,53 @@
+Require Import Resources.utility.
+Require Import Resources.name.
+Require Import Resources.type.
+Require Import Resources.value.
+
+
+(** Memory model  *)
+Definition LocalMemory : Set := LocalVariable ⇀ RuntimeValue.
+
+Module StructSig.
+Record StructSig := {
+  kind : Kind;
+  field: list (FieldName * NonReferenceType)
+}.
+End StructSig.
+Import StructSig(StructSig).
+
+Record Module : Set := {
+  struct_decls : StructName ⇀ StructSig;
+}.
+
+Record Account : Set := {
+  resources : StructID ⇀ Resource;
+  modules : ModuleName ⇀ Module
+}.
+
+Definition GlobalMemory : Set := AccountAddress ⇀ Account.
+
+Record Memory := {
+  local: LocalMemory;
+  global: GlobalMemory;
+}.
+
+Definition mem_remove (M : Memory) (x : LocalVariable) : Memory.
+Admitted.
+
+Definition mem_update_local (M : Memory) (x : LocalVariable) (v : RuntimeValue) : Memory.
+Admitted.
+
+Definition mem_update_ref (M : Memory) (r : Reference) (v : RuntimeValue) : Memory.
+Admitted.
+
+Inductive maps_var_to : Memory → LocalVariable → RuntimeValue → Prop :=.
+
+Inductive maps_ref_to : Memory → Reference → RuntimeValue → Prop :=.
+
+Inductive maps_struct_kind : Memory → StructType → Kind → Prop :=.
+
+Inductive maps_struct_arity : Memory → StructType → nat → Prop :=.
+
+Definition LocalStack : Set := list RuntimeValue.
+
+Inductive fresh_tag (M : Memory) (S : LocalStack) : Tag → Prop :=.
