name.v
@@ -1,0 +1,26 @@
+Require Import Coq.Unicode.Utf8_core.
+Require Import Resources.utility.
+
+(** Names  *)
+Parameter LocalVariable : Set.
+Parameter var_dec_eq :  ∀ (x y : LocalVariable), {x = y} + {x <> y}.
+Instance var_eq_dec : EqDec LocalVariable := {
+  eq_dec := var_dec_eq
+}.
+
+Parameter FieldName : Set.
+Parameter StructName : Set.
+Parameter ModuleName : Set.
+Parameter AccountAddress : Set.
+
+Record ModuleID : Set := {
+  account_addr : AccountAddress;
+  module_name : ModuleName;
+}.
+
+Record StructID : Set := {
+  mod_id : ModuleID;
+  name : StructName;
+}.
+
+Definition GlobalResourceID := StructID.
