type.v
@@ -1,0 +1,26 @@
+Require Import Resources.name.
+(** Types *)
+Inductive Kind : Set := resourceKind | unrestrictedKind.
+
+Module StructType.
+Record StructType : Set := {
+  struct_id : StructID;
+}.
+End StructType.
+Export StructType(StructType).
+
+Inductive PrimitiveType : Set :=
+  | accountAddressType : PrimitiveType
+  | signerType : PrimitiveType
+  | boolType : PrimitiveType
+  | unsignedInt64Type : PrimitiveType
+  | bytesType : PrimitiveType.
+
+Inductive NonReferenceType : Set :=
+  | structNonReferenceType : StructType -> NonReferenceType
+  | primitiveNonReferenceType : PrimitiveType -> NonReferenceType.
+
+Inductive MoveType : Set :=
+  | nonReferenceMoveType : NonReferenceType -> MoveType
+  | mutRefMoveType : NonReferenceType -> MoveType
+  | refMoveType : NonReferenceType -> MoveType.
