utility.v
@@ -1,0 +1,24 @@
+Require Export Coq.Unicode.Utf8_core.
+(** Utility *)
+Notation "A ⇀ B" := (A → option B) (at level 75, right associativity).
+
+Inductive maps_to : ∀ {A B : Set} (f : A ⇀ B) (x : A) (y : B), Prop :=
+  maps_to_ : ∀ {A B : Set} (f : A ⇀ B) (x : A) (y : B),
+    f x = Some(y) →
+    maps_to f x y.
+
+Class EqDec (A : Type) := {
+  eq_dec : ∀ (x y : A), {x = y} + {x <> y}
+}.
+
+Definition remove {X : Set} {Y : Set} `{eq : EqDec X} (f : X ⇀ Y) (a : X) : X ⇀ Y :=
+  fun x => match eq_dec x a with
+    | left _ => None
+    | right _ => f x
+    end.
+
+Definition update {X : Set} {Y : Set} `{eq : EqDec X} (f : X ⇀ Y) (a : X) (b : Y) : X ⇀ Y :=
+  fun x => match eq_dec x a with
+    | left _ => Some(b)
+    | right _ => f x
+    end.
