value.v
@@ -1,0 +1,118 @@
+Require Import Coq.Lists.List.
+Open Scope list_scope.
+Import ListNotations.
+Require Import Resources.utility.
+Require Import Resources.name.
+Require Import Resources.type.
+(** Values *)
+Parameter Signer : Set.
+Parameter UnsignedInt64 : Set.
+Parameter Bytes : Set.
+
+Parameter Tag : Set.
+
+Parameter tag_dec_eq :  ∀ (x y : Tag), {x = y} + {x <> y}.
+Instance tag_eq_dec : EqDec Tag := {
+  eq_dec := tag_dec_eq
+}.
+
+Inductive Resource : Set :=
+  | resource : Tag → StructType → list Value -> Resource
+
+with Struct : Set :=
+  | struct : StructType → list Value -> Struct
+
+with PrimitiveValue : Set :=
+  | accountAddressValue : AccountAddress -> PrimitiveValue
+  | signerValue : Signer -> PrimitiveValue
+  | boolValue : bool -> PrimitiveValue
+  | unsignedInt64Value : UnsignedInt64 -> PrimitiveValue
+  | bytesValue : Bytes -> PrimitiveValue
+
+with UnrestrictedValue : Set :=
+  | structValue : Struct -> UnrestrictedValue
+  | primitiveValue : PrimitiveValue -> UnrestrictedValue
+
+with Value : Set :=
+  | resourceValue : Resource -> Value
+  | unrestrictiveValue : UnrestrictedValue -> Value.
+
+Definition tag_of (r : Resource) : Tag :=
+  match r with
+  | resource t _ _ => t
+  end.
+
+Coercion structValue : Struct >-> UnrestrictedValue.
+Coercion resourceValue : Resource >-> Value.
+Coercion unrestrictiveValue : UnrestrictedValue >-> Value.
+Coercion primitiveValue : PrimitiveValue >-> UnrestrictedValue.
+Coercion boolValue : bool >-> PrimitiveValue.
+Coercion unsignedInt64Value : UnsignedInt64 >-> PrimitiveValue.
+Coercion accountAddressValue : AccountAddress >-> PrimitiveValue.
+Coercion bytesValue : Bytes >-> PrimitiveValue.
+
+(** References  *)
+Inductive Qualifier : Set :=
+  | mut : Qualifier
+  | immut : Qualifier.
+
+Inductive Root : Set :=
+  | local_root : LocalVariable -> Root
+  | global_root : GlobalResourceID -> Root.
+
+Coercion local_root : LocalVariable >-> Root.
+Coercion global_root : GlobalResourceID >-> Root.
+
+Definition Path := list FieldName.
+
+Parameter read_val : Value → Path → Value → Prop.
+
+Axiom read_unrestricted : ∀ (u : UnrestrictedValue) (p : Path) (v : Value),
+  read_val u p v →
+  ∃ (u' : UnrestrictedValue), v = u'.
+
+Axiom read_resource : ∀ (s : Value) (p : Path) (a : Resource),
+read_val s p a →
+∃ (b : Resource), s = b.
+
+Record Reference : Set := {
+  root : Root;
+  access_path : Path;
+  mutability : Qualifier;
+}.
+
+Inductive is_mut : Reference → Prop :=
+  | is_mut_ref : ∀ (r : Root) (p : Path), is_mut {|
+    root := r; access_path := p; mutability := mut;
+  |}.
+
+Inductive is_immut : Reference → Prop :=
+  | is_immut_ref : ∀ (r : Root) (p : Path), is_immut {|
+  root := r; access_path := p; mutability := immut;
+  |}.
+
+Definition extend_ref (r : Reference) (e : FieldName) : Reference :=
+  match r with
+  | {| root := root ; access_path := access_path; mutability := mutability |} => {|
+    root := root;
+    access_path := access_path ++ [ e ];
+    mutability := mutability;
+  |}
+  end.
+
+Definition freeze_ref (r : Reference) : Reference :=
+  match r with
+  | {| root := root; access_path := access_path; mutability := _ |} => {|
+      root := root;
+      access_path := access_path;
+      mutability := immut;
+  |}
+  end.
+
+Inductive RuntimeValue : Set :=
+  | val : Value → RuntimeValue
+  | ref_val : Reference → RuntimeValue.
+
+Coercion val : Value >-> RuntimeValue.
+Coercion ref_val : Reference >-> RuntimeValue.
+Coercion foo (v : UnrestrictedValue) := val (unrestrictiveValue v).
