Makefile
@@ -1,0 +1,14 @@
+MODULES := utility name type value memory instr resources
+VS := $(MODULES:%=%.v)
+
+.PHONY: coq clean
+
+coq: Makefile.coq
+	$(MAKE) -f Makefile.coq
+
+Makefile.coq: Makefile $(VS)
+	coq_makefile -R . Resources $(VS) -o Makefile.coq
+
+clean:: Makefile.coq
+	$(MAKE) -f Makefile.coq clean
+	rm -f Makefile.coq
